@prefix xsd:  <http://www.w3.org/2001/XMLSchema#> .
@prefix rdf:  <http://www.w3.org/1999/02/22-rdf-syntax-ns#> .
@prefix rdfs: <http://www.w3.org/2000/01/rdf-schema#> .
@prefix owl: <http://www.w3.org/2002/07/owl#> .

@prefix dcterms: <http://purl.org/dc/terms/>.
@prefix skos: <http://www.w3.org/2004/02/skos/core#>.
@prefix foaf: <http://xmlns.com/foaf/0.1/>.
@prefix sioc: <http://rdfs.org/sioc/ns#>.
@prefix doap: <http://usefulinc.com/ns/doap#>.

@prefix vs: <http://www.w3.org/2003/06/sw-vocab-status/ns#>.
@prefix vann: <http://purl.org/vocab/vann/>.
@prefix http: <http://www.w3.org/2006/http#>.
@prefix prv: <http://purl.org/net/provenance/ns#> .

@prefix pingback: <http://purl.org/net/pingback/> .
@prefix dssn: <http://purl.org/net/dssn/> .


###
# DSSN classes
###

dssn:Application a owl:Class;
    rdfs:isDefinedBy <http://purl.org/net/dssn/>;
    vs:term_status "unstable";
    rdfs:subClassOf foaf:Agent;
    owl:disjointWith foaf:Person;
    rdfs:comment "An application on the web, which can act in the name of a WebID owner (access delegation)";
    rdfs:label "application".

###
# DSSN properties
###

dssn:activityFeed a owl:ObjectProperty;
    rdfs:isDefinedBy <http://purl.org/net/dssn/>;
    vs:term_status "unstable";
    rdfs:domain foaf:Agent;
    rdfs:subPropertyOf sioc:feed;
    rdfs:comment "link a agent / person to an activity feed";
    rdfs:label "activity feed".

dssn:syncFeed a owl:ObjectProperty;
    rdfs:isDefinedBy <http://purl.org/net/dssn/>;
    vs:term_status "unstable";
    rdfs:subPropertyOf sioc:feed;
    rdfs:comment "link a resource to a changeset / history feed";
    rdfs:label "sync feed".

dssn:trustedService a owl:ObjectProperty;
    rdfs:isDefinedBy <http://purl.org/net/dssn/>;
    vs:term_status "unstable";
    rdfs:domain foaf:Agent;
    rdfs:comment "A service which should be used by applications, since the owner of the WebID trusts owner of the service.";
    rdfs:label "trusted service".

dssn:searchService a owl:ObjectProperty;
    rdfs:isDefinedBy <http://purl.org/net/dssn/>;
    vs:term_status "unstable";
    rdfs:subPropertyOf dssn:trustedService;
    rdfs:comment "A (trusted and WebID protocol enabled) private SPARQL search service, which should be used by applications which act in the name of the owner of the WebID.";
    rdfs:label "search service".

dssn:updateService a owl:ObjectProperty;
    rdfs:isDefinedBy <http://purl.org/net/dssn/>;
    vs:term_status "unstable";
    rdfs:subPropertyOf dssn:trustedService;
    rdfs:comment "A (trusted and WebID protocol enabled) private SPARQL update service, which should be used by applications which act in the name of the owner of the WebID.";
    rdfs:label "update service".

###
# Example
###


###
# Vocabulary description and documentation
###

<http://purl.org/net/dssn/> a owl:Ontology;
    foaf:maker <http://sebastian.tramp.name>,
        <http://philipp.frischmuth24.de/id/me>,
        <http://www.informatik.uni-leipzig.de/~auer/foaf.rdf#me>;
    doap:maintainer <http://sebastian.tramp.name>;
    vann:preferredNamespacePrefix "dssn";
    vann:preferredNamespaceUri "http://purl.org/net/dssn/";
    foaf:homepage <http://aksw.org/>;
    #vann:example <http://aksw.org/Projects/SemanticPingback#usagefoaf>, <http://aksw.org/Projects/SemanticPingback#HowTo>, <http://aksw.org/Projects/SemanticPingback#Implementations>;
    #vann:changes <http://code.google.com/p/ontowiki/source/list?path=/SemanticPingback/namespace.rdf&amp;repo=models>;
    rdfs:label "DSSN Vocabulary";
    skos:note "vocabulary to describe some Distributed Semantic Social Network relations ...".

#<http://aksw.org/Projects/SemanticPingback> a foaf:Document;
#    rdfs:label "Semantic Pingback Project Homepage".


<http://www.informatik.uni-leipzig.de/~auer/foaf.rdf#me> a foaf:Person; foaf:name "SÃ¶ren Auer".
<http://philipp.frischmuth24.de/id/me> a foaf:Person; foaf:name "Philipp Frischmuth".
<http://sebastian.tramp.name> a foaf:Person; foaf:name "Sebastian Tramp".

